bruh

Hashtable.dfy
@@ -2,45 +2,62 @@ datatype List<T> = Nil | Cons(head: T,tail: List<T>)
 datatype Option<T> = None | Some(elem: T)
 
 class Hashtable<K(==,!new),V(!new)> {
-    var size : int;
-    var data : array<List<(K,V)>>;
-    
-    function hash(key: K) : int
-    
-    function bucket(k: K,n: int) : int
-    
-    constructor(n: int)
+  var size : int;
+  var data : array<List<(K,V)>>;
 
-    method clear()
+  function hash(key: K) : int
 
-    method resize()
+  function bucket(k: K,n: int) : int
+    requires n > 0
+  {
+    hash(k) % n
+  }
 
-    function list_find (k:K, l:List<(K,V)>) : option<V>
-        ensures match list_find(k,l) {
-            case None => forall v :: !mem((k,v),l)
-            case Some(v) => mem((k,v),l)
-        }
-    {
-        match l {
-            case Nil => None
-            case Cons((k`,v),xs) => if k=k` then Some(v) else list_find(k,xs)        
-        }
+  constructor(n: int)
+    requires n > 0
+  {
+    size := n;
+    data := new List<(K,V)>[n];
+  }
+
+  method clear()
+
+  method resize()
+
+  function mem<T(==)> (k: T, l: List<T>) : bool
+  {
+    match l
+    case Nil => false
+    case Cons(k', t) =>
+      if(k' == k) then true else mem(k, t)
+  }
+
+  function list_find (k:K, l:List<(K,V)>) : Option<V>
+    ensures match list_find(k,l) {
+              case None => forall v :: !mem((k,v),l)
+              case Some(v) => mem((k,v),l)
+            }
+  {
+    match l {
+      case Nil => None
+      case Cons((k',v),xs) => if k==k' then Some(v) else list_find(k,xs)
     }
+  }
 
-    method find(k: K) returns (r: Option<V>)
+  method find(k: K) returns (r: Option<V>)
 
-    function list_remove(k: K,l: List<(K,V)>) : List<(K,V)>
-        decreases l
-        ensures forall k` , v :: mem((k`,v),list_remove(k,l)) <==> (mem((k`,v),l) && k` != k)
-    {
-        match l {
-            case Nil ⇒ Nil
-            case Cons((k`,v),xs) => if k=k` then list_remove(k,xs) else
-            Cons((k`,v),list_remove(k,xs))
-        }
+  function list_remove(k: K,l: List<(K,V)>) : List<(K,V)>
+    decreases l
+    ensures forall k' , v :: mem((k',v),list_remove(k,l)) <==> (mem((k',v),l) && k' != k)
+  {
+    match l {
+      case Nil => Nil
+      case Cons((k',v),xs) => if k==k' then list_remove(k,xs) else
+      Cons((k',v),list_remove(k,xs))
     }
+  }
 
-    method remove(k: K)
+  method remove(k: K)
 
-    method add(k: K,v: V)
+  method add(k: K,v: V)
 }
